theories/abs_functional_metatheory.v
@@ -1,26 +1,677 @@
-From ABS Require Import abs_defs.
-From Coq Require Import List.
+From ABS Require Import abs_defs
+  utils.
+
+From Coq Require Import List
+  FSets.FMapFacts
+  Lia.
+
+From Equations Require Import Equations.
+
+Require Import FMapList.
+Module MapFacts := FSets.FMapFacts.Facts Map.
 Import ListNotations.
 
 (** * ABS Functional Metatheory *)
 
+Section FunctionalMetatheory.
+
+Hypothesis (vars_fs_distinct: forall (x_:x) (fn_:fn), x_ <> fn_).
+Hypothesis (vars_well_typed: forall (x_:x) (G0: G) T0,
+             Map.find x_ G0 = Some T0 ->
+             exists T_, T0 = ctxv_T T_).
+
 Definition subG (G1 G2 : G) : Prop :=
-  forall (key : string) (elt : ctxv), 
+  forall (key : string) (elt : ctxv),
     Map.find key G1 = Some elt ->
     Map.find key G2 = Some elt.
 
+Notation "G ⊢ e : T" := (typ_e G e T) (at level 5).
+Notation "G F⊢ F" := (typ_F G F) (at level 5).
+Notation "G1 ⊆ G2" := (subG G1 G2) (at level 5).
+
+Lemma subG_refl: forall G0,
+  subG G0 G0.
+Proof. easy. Qed.
+
+Lemma subG_add: forall G0 G1 y T_,
+  subG G0 G1 ->
+  ~ Map.In y G0 ->
+  subG G0 (Map.add y T_ G1).
+Proof.
+  intros.
+  intros ?x_ ?T_ ?.
+
+  destruct (eq_x y x_); subst.
+  - exfalso.
+    apply H0.
+    apply MapFacts.in_find_iff.
+    intro.
+    rewrite H1 in H2.
+    discriminate.
+  - apply Map.find_1.
+    apply MapFacts.add_neq_mapsto_iff; auto.
+    pose proof H x_ T_0 H1.
+    apply Map.find_2.
+    assumption.
+Qed.
+
+Lemma subG_add_2: forall G0 G1 y T_,
+  subG G0 G1 ->
+  Map.find y G0 = Some T_ ->
+  subG G0 (Map.add y T_ G1).
+Proof.
+  intros.
+  intros ?x_ ?T_ ?.
+
+  destruct (eq_x y x_); subst.
+  - rewrite H0 in H1.
+    inv H1.
+    apply Map.find_1.
+    now apply Map.add_1.
+  - apply Map.find_1.
+    apply MapFacts.add_neq_mapsto_iff; auto.
+    pose proof H x_ T_0 H1.
+    apply Map.find_2.
+    assumption.
+Qed.
+
+(* this is stricter than the ABS paper *)
+(* we require that any variables in the typing context also exist in the state *)
 Definition G_vdash_s (G5 : G) (s5 : s) :=
- forall (x5 : x) (t5 : t) (T5 : T),
-  Map.find x5 s5 = Some t5 ->
+ forall (x5 : x) (T5 : T),
   Map.find x5 G5 = Some (ctxv_T T5) ->
-  typ_e G5 (e_t t5) T5.
+  exists t5,
+  Map.find x5 s5 = Some t5 /\ typ_e G5 (e_t t5) T5.
+
+Notation "G1 G⊢ s1" := (G_vdash_s G1 s1) (at level 5).
+
+Lemma fresh_subG: forall G0 s0 (sub_list: list (T*x*t*x)),
+  G_vdash_s G0 s0 ->
+  fresh_vars_s (map (fun '(_,_,_,y)=>y) sub_list) s0 ->
+  NoDup (map (fun '(_,_,_,y)=>y) sub_list) ->
+  subG G0 (fold_right (fun '(T_,_,_,y_) G0 => Map.add y_ (ctxv_T T_) G0) G0 sub_list).
+Proof.
+  intros.
+  induction sub_list.
+  - easy.
+  - destruct a as (((?T_, ?x_), ?t_), y).
+    inv H1.
+    inv H0.
+    pose proof IHsub_list H2 H5.
+    cbn.
+    apply subG_add; auto.
+    intro.
+
+    apply MapFacts.in_find_iff in H3.
+    apply MapFacts.not_find_in_iff in H1.
+    pose proof map_neq_none_is_some _ _ H3 as (?T_, ?).
+    pose proof vars_well_typed _ _ _ H6 as (?T_, ->).
+    pose proof H _ _ H6 as (?t_, (?, _)).
+    rewrite H1 in H7.
+    discriminate.
+Qed.
+
+Lemma fresh_consistent: forall G0 s0 (sub_list: list (T*x*t*x)),
+  G_vdash_s G0 s0 ->
+  (forall T_ t_, In (T_, t_) (map (fun '(T_, _, t_, _) => (T_, t_)) sub_list) ->
+            typ_e G0 (e_t t_) T_) ->
+  fresh_vars_s (map (fun '(_,_,_,y)=>y) sub_list) s0 ->
+  NoDup (map (fun '(_,_,_,y)=>y) sub_list) ->
+  G_vdash_s (fold_right (fun '(T_,_,_,y_) G0 => Map.add y_ (ctxv_T T_) G0) G0 sub_list)
+    (fold_right (fun '(_,_,t_,y_) s0 => Map.add y_ t_ s0) s0 sub_list).
+Proof.
+  intros.
+  induction sub_list.
+  * easy.
+  * destruct a as (((?T_, ?x_), ?t_), y).
+    inv H1.
+    inv H2.
+
+    cbn.
+    intros ?y ?T_ ?.
+    destruct (eq_x y y0); subst.
+  - exists t_.
+    split...
+    + apply Map.find_1.
+      now apply Map.add_1.
+    + assert (T_ = T_0).
+      {
+        apply Map.find_2 in H1.
+        apply MapFacts.add_mapsto_iff in H1.
+        destruct H1 as [(_, ?) | (?, ?)].
+        + now inv H1.
+        + exfalso.
+          now apply H1.
+      }
+      assert (In (T_0, t_) (map (fun '(T_, _, t_, _) => (T_, t_)) ((T_, x_, t_, y0) :: sub_list)))
+        by (left; now rewrite H2).
+      specialize (H0 _ _ H5).
+      inv H0; constructor.
+  - apply Map.find_2 in H1.
+    apply Map.add_3 in H1; auto.
+    apply Map.find_1 in H1.
+    assert (forall (T_ : T) (t_ : t),
+             In (T_, t_) (map (fun '(T_0, _, t_0, _) => (T_0, t_0)) sub_list) ->
+             typ_e G0 (e_t t_) T_).
+    {
+      intros.
+      apply H0.
+      right.
+      assumption.
+    }
+    pose proof IHsub_list H2 H4 H7 _ _ H1 as (?t_, (?, ?)).
+    exists t_0.
+    split...
+    + apply Map.find_1.
+      apply Map.add_2; auto.
+      apply Map.find_2; assumption.
+    + inv H8; constructor.
+Qed.
+
+Lemma subG_consistent: forall G1 G2 s0,
+  subG G1 G2 -> G_vdash_s G2 s0 -> G_vdash_s G1 s0.
+Proof.
+  intros.
+  intros x_ t_ ?.
+
+  pose proof H _ _ H1.
+  pose proof H0 _ _ H2 as (?t, (?, ?)).
+  exists t.
+  split; auto.
+  inv H4;constructor.
+Qed.
+
+Lemma subG_type: forall G1 G2 e0 T0,
+  subG G1 G2 -> typ_e G1 e0 T0 -> typ_e G2 e0 T0.
+Proof.
+  intros.
+  induction H0.
+  - constructor.
+  - constructor.
+  - apply H in H0.
+    constructor.
+    apply H0.
+  - constructor.
+    + intros.
+      apply H1; auto.
+    + apply H in H2.
+      apply H2.
+Qed.
+
+(* this is 9.3.8 from Types and Programming Languages *)
+(* it has not yet proven useful *)
+Lemma subst_lemma_one_alt: forall (x0 x1:x) G0 e0 T0 T1,
+  typ_e (Map.add x0 (ctxv_T T1) G0) e0 T0 ->
+  typ_e G0 (e_var x1) T1 ->
+  typ_e G0 (e_var_subst_one e0 x0 x1) T0.
+Proof.
+  intros.
+  generalize dependent T0.
+  generalize dependent T1.
+  generalize dependent G0.
+  eapply e_ott_ind with
+      (n:=e0)
+      (P_list_e:= fun e_list => forall e0,
+                    In e0 e_list ->
+                    forall G0 T0 T1,
+                    typ_e (Map.add x0 (ctxv_T T1) G0) e0 T0 ->
+                    typ_e G0 (e_var x1) T1 ->
+                    typ_e G0 (e_var_subst e0 [(x0, x1)]) T0)
+  ;cbn; intros.
+  - inv H; simp e_var_subst_one; constructor.
+  - inv H.
+    simp e_var_subst_one.
+    destruct (eq_x x5 x0); subst.
+    + apply Map.find_2 in H3.
+      apply MapFacts.add_mapsto_iff in H3.
+      destruct H3 as [(?&?) | (?&?)]; subst.
+      * inv H1.
+        assumption.
+      * contradiction.
+    + constructor.
+      apply Map.find_1.
+      eapply Map.add_3.
+      * apply not_eq_sym.
+        apply n.
+      * apply Map.find_2 in H3.
+        apply H3.
+  - inv H1.
+    simp e_var_subst_one.
+    rewrite <- subst_fst_commute.
+    replace (map (fun x : e * T => let (e_, _) := let '(e_, T_) := x in (e_var_subst_one e_ x0 x1, T_) in e_) e_T_list)
+      with
+        (map (fun pat_ : e * T => let (e_, _) := pat_ in e_)
+           (map (fun '(e_, T_) => (e_var_subst_one e_ x0 x1, T_)) e_T_list))
+    by apply map_map.
+    constructor.
+    + rewrite map_map.
+      intros.
+      apply in_map_iff in H1.
+      destruct H1 as ((?e_&?T_) & ? & ?).
+      inv H1.
+      eapply H.
+      * apply in_map_iff.
+        exists (e_0, T_).
+        split; eauto.
+      * apply H5.
+        apply in_map_iff.
+        exists (e_0, T_).
+        split; auto.
+      * apply H0.
+    + apply Map.find_1.
+      apply Map.find_2 in H7.
+      rewrite subst_snd_commutes.
+      eapply Map.add_3; eauto.
+  - inv H.
+  - inv H1.
+    + eapply H; eauto.
+    + eapply H0; eauto.
+Qed.
+
+Lemma same_type_sub: forall (sub_list: list (x*x)) G0 e0 T0,
+    typ_e G0 e0 T0 ->
+    (forall x0 y0 T0,
+      In (x0, y0) sub_list ->
+      Map.find x0 G0 = Some T0 ->
+      Map.find y0 G0 = Some T0) ->
+    typ_e G0 (e_var_subst e0 sub_list) T0.
+Proof.
+  {
+  intros.
+  generalize dependent T0.
+  eapply e_ott_ind with
+      (n:= e0)
+      (P_list_e:= fun e_list => forall e0 T0,
+                    In e0 e_list ->
+                    typ_e G0 e0 T0 ->
+                    typ_e G0 (e_var_subst e0 sub_list) T0)
+  ; intros.
+  - rewrite subst_term.
+    simp e_var_subst_one.
+  - rewrite subst_var.
+    constructor.
+    induction sub_list.
+    + inv H.
+      now simpl.
+    + destruct a.
+      simpl.
+      destruct (eq_x (replace_var x5 sub_list) x); subst.
+      * eapply H0; eauto.
+        -- now left.
+        -- apply IHsub_list; eauto.
+           intros.
+           eapply H0; eauto.
+           now right.
+      * eapply IHsub_list; eauto.
+        intros.
+        eapply H0; eauto.
+        now right.
+  - inv H1.
+    rewrite subst_fn.
+    rewrite map_map.
+    replace (map (fun x : e * T => e_var_subst (let (e_, _) := x in e_) sub_list) e_T_list)
+      with (map (fun pat_:e*T => let (e, _) := pat_ in e) (map (fun '(e, T) => (e_var_subst e sub_list, T)) e_T_list))
+      by (rewrite map_map; apply map_ext; now intros (?, ?)).
+    constructor.
+    + intros.
+      apply in_map_iff in H1.
+      destruct H1 as ((?e, ?T), (?, ?)).
+      inv H1.
+      apply in_map_iff in H2.
+      destruct H2 as ((?e_, ?T_), (?, ?)).
+      inv H1.
+      apply H.
+      * apply in_map_iff.
+        exists (e_0, T_).
+        split; eauto.
+      * apply H5.
+        apply in_map_iff.
+        exists (e_0, T_).
+        split; eauto.
+    + now replace (map (fun pat_ : e * T => let (_, T_) := pat_ in T_) (map (fun '(e, T) => (e_var_subst e sub_list, T)) e_T_list))
+        with(map (fun pat_ : e * T => let (_, T_) := pat_ in T_) e_T_list)
+      by (rewrite map_map; apply map_ext; now intros (?, ?)).
+  - inv H.
+  - inv H2.
+    + now apply H.
+    + now apply H1.
+  }
+
+Qed.
+
+Lemma subst_lemma_one: forall G0 x0 y0 e0 Ai A,
+  typ_e (Map.add x0 Ai G0) e0 A ->
+  fresh_vars_e [y0] e0 ->
+  typ_e (Map.add y0 Ai G0) (e_var_subst_one e0 x0 y0) A.
+Proof.
+  {
+    intros.
+    generalize dependent A.
+    revert H0.
+    apply e_ott_ind with
+        (n:=e0)
+        (P_list_e:= fun e_list =>
+                      forall e0 A,
+                      In e0 e_list ->
+                      fresh_vars_e [y0] e0 ->
+                      typ_e (Map.add x0 Ai G0) e0 A ->
+                      typ_e (Map.add y0 Ai G0) (e_var_subst_one e0 x0 y0) A);
+      intros.
+    - simp e_var_subst_one.
+      inv H; constructor.
+    - simp e_var_subst_one.
+      inv H.
+      apply Map.find_2 in H3.
+      apply MapFacts.add_mapsto_iff in H3.
+      destruct H3 as [(?,?)|(?,?)]; subst.
+      + destruct (eq_x x5 x5); subst.
+        * constructor.
+          apply Map.find_1.
+          now apply Map.add_1.
+        * contradiction.
+
+      + destruct (eq_x x5 x0); subst.
+        * contradiction.
+        * destruct (eq_x x5 y0); subst.
+          -- simp fresh_vars_e in H0.
+             exfalso.
+             apply H0.
+             now left.
+          -- constructor.
+             apply Map.find_1.
+             apply Map.add_2; eauto.
+    - simp e_var_subst_one.
+      inv H1.
+      replace (e_list_subst_one (map (fun pat_ : e * T => let (e_, _) := pat_ in e_) e_T_list) x0 y0)
+        with (map (fun pat_:e*T => let (e, _) := pat_ in e) (map (fun '(e, T) => (e_var_subst_one e x0 y0, T)) e_T_list))
+        by (rewrite e_list_subst_map;
+            rewrite 2 map_map;
+            apply map_ext;
+            now intros (?,?)).
+      constructor.
+      + intros.
+        apply in_map_iff in H1.
+        destruct H1 as ((?e, ?T), (?, ?)).
+        inv H1.
+        apply in_map_iff in H2.
+        destruct H2 as ((?e_, ?T_), (?, ?)).
+        inv H1.
+        apply H.
+        * apply in_map_iff.
+          exists (e_0, T_).
+          split; eauto.
+        * simp fresh_vars_e in H0.
+          eapply e_list_fresh.
+          apply H0.
+          apply in_map_iff.
+          eexists (e_0, T_).
+          split; auto.
+        * apply H5.
+          apply in_map_iff.
+          exists (e_0, T_).
+          split; eauto.
+      + replace (map (fun pat_ : e * T => let (_, T_) := pat_ in T_) (map (fun '(e, T) => (e_var_subst_one e x0 y0, T)) e_T_list))
+          with(map (fun pat_ : e * T => let (_, T_) := pat_ in T_) e_T_list)
+          by (rewrite map_map; apply map_ext; now intros (?, ?)).
+
+        apply Map.find_2 in H7.
+        apply MapFacts.add_mapsto_iff in H7.
+        destruct H7 as [(?,?)|(?,?)].
+        * exfalso.
+          apply (vars_fs_distinct _ _ H1).
+        * apply Map.find_1.
+          apply Map.add_2; eauto.
+    - inv H.
+    - destruct H1; subst.
+      + apply H; eauto.
+      + apply H0; eauto.
+  }
+Qed.
+
+Lemma subst_lemma: forall (T_x_t_y_list:list (T*x*t*x)) G0 e0 A,
+  typ_e (fold_right (fun '(Ai, x_, _, _) (G0 : G) => Map.add x_ (ctxv_T Ai) G0) G0 T_x_t_y_list) e0 A ->
+  NoDup (map (fun '(_, _, _, y) => y) T_x_t_y_list) ->
+  NoDup (map (fun '(_, x, _, _) => x) T_x_t_y_list) ->
+  fresh_vars_e (map (fun '(_, _, _, y) => y) T_x_t_y_list) e0 ->
+  disjoint (map (fun '(_, _, _, y) => y) T_x_t_y_list) (map (fun '(_, x, _, _) => x) T_x_t_y_list) ->
+  typ_e (fold_right (fun '(Ai, _, _, y) (G0 : G) => Map.add y (ctxv_T Ai) G0) G0 T_x_t_y_list)
+    (e_var_subst e0 (map (fun '(_, x_, _, y_) => (x_, y_)) T_x_t_y_list)) A.
+Proof.
+  intros.
+  generalize dependent G0.
+  generalize dependent e0.
+  induction T_x_t_y_list; intros.
+  - easy.
+  - destruct a as (((?T_,?x_),?t_),?y).
+    unfold e_var_subst.
+    simpl in *.
+    inv H0.
+    inv H1.
+    pose proof fresh_first_e _ _ _ H2.
+    pose proof fresh_monotone_e _ _ _ H2.
+    epose proof disjoint_monotone _ _ _ _ H3.
+    assert (~ In x_ (map (fun '(_, y) => y) (map (fun '(Ai, _, _, y1) => (Ai, y1)) T_x_t_y_list))).
+    { intro.
+      apply (H3 x_).
+      - right.
+        rewrite map_map in H9.
+        replace (map (fun '(_, _, _, y1) => y1) T_x_t_y_list)
+          with
+            (map (fun x0 : T * x * t * x => let '(_, y) := let '(Ai, _, _, y1) := x0 in (Ai, y1) in y) T_x_t_y_list).
+        apply H9.
+        apply map_eq.
+        now intros (((?, ?), ?), ?).
+      - now left.
+    }
+    replace (Map.add x_ (ctxv_T T_) (fold_right (fun '(Ai, x_, _, _) (G0 : G) => Map.add x_ (ctxv_T Ai) G0) G0 T_x_t_y_list))
+      with (fold_right (fun '(Ai, x_, _, _) (G0 : G) => Map.add x_ (ctxv_T Ai) G0) (Map.add x_ (ctxv_T T_) G0) T_x_t_y_list)
+      in H.
+    pose proof IHT_x_t_y_list H7 H8 H4 _ H1 _ H as IH.
+    replace (fold_right (fun '(Ai, _, _, y) (G0 : G) => Map.add y (ctxv_T Ai) G0) (Map.add x_ (ctxv_T T_) G0) T_x_t_y_list)
+      with (Map.add x_ (ctxv_T T_) (fold_right (fun '(Ai, _, _, y) (G0 : G) => Map.add y (ctxv_T Ai) G0) G0 T_x_t_y_list))
+      in IH.
+    assert (fresh_vars_e [y] (e_var_subst e0 (map (fun '(_, x_, _, y_) => (x_, y_)) T_x_t_y_list))).
+    {
+      assert (map snd (map (fun '(_, x_0, _, y_) => (x_0, y_)) T_x_t_y_list) = map (fun '(_, _, _, y) => y) T_x_t_y_list).
+      {
+        rewrite map_map.
+        apply map_eq.
+        now intros (((?, ?), ?), ?).
+      }
+      apply fresh_var_subst; try rewrite H10; auto.
+    }
+    now apply (subst_lemma_one _ _ _ _ _ _ IH H10).
+
+    (* resolving those replaces from earlier *)
+    {
+      epose proof fold_add_comm G0 x_ T_ (map (fun '(Ai, _, _, y1) => (Ai, y1)) T_x_t_y_list) H9.
+      rewrite 2 fold_map1.
+      Fail apply H10.
+      (* why? *)
+      admit.
+    }
+    {
+      epose proof fold_add_comm G0 x_ T_ (map (fun '(Ai, _, _, y1) => (Ai, y1)) T_x_t_y_list) H9.
+      rewrite 2 fold_map2.
+      Fail rewrite <- H10.
+      (* why? *)
+      admit.
+    }
+Admitted.
 
 Lemma type_preservation : forall (Flist : list F) (G5 : G) (s5 : s),
-  (* FIXME: add well-typing of all function definitions here *)
   G_vdash_s G5 s5 ->
+  Forall (typ_F G5) Flist ->
   forall (e5 : e) (T5 : T) (s' : s) (e' : e),
     typ_e G5 e5 T5 ->
     red_e Flist s5 e5 s' e' ->
     exists G', subG G5 G' /\ G_vdash_s G' s' /\ typ_e G' e' T5.
 Proof.
-Admitted.
+  intros Fs G5 s0 s_well_typed F_well_typed.
+  intros e0 T0 s' e' e0_type reduction.
+  generalize dependent T0.
+  generalize dependent G5.
+  induction reduction.
+  - intros.
+    exists G5; splits.
+    1,2: easy.
+    inv e0_type.
+    destruct (s_well_typed x5 T0 H2) as (?, (?, ?)).
+    rewrite H in H0.
+    inv H0.
+    assumption.
+
+  - (* RED_FUN_EXPR *)
+    intros.
+    inv e0_type.
+    rewrite app_nil_r in H0.
+    pose proof split_corresponding_list e_T_list e_list e_5 e'_list H0
+      as (T_list & T_5 & T'_list & ? & ? & ?).
+    assert (In (e_5, T_5) (map (fun pat_ : e * T => let (e_0, T_0) := pat_ in (e_0, T_0)) e_T_list)). {
+      rewrite H3.
+      apply in_map_iff.
+      exists (e_5, T_5).
+      split; auto.
+      apply in_combine_split with (2:=eq_refl); auto.
+    }
+    pose proof H2 e_5 T_5 H5.
+    destruct (IHreduction G5 s_well_typed F_well_typed _ H6) as (G' & G'extends & G'consistent & ?).
+    exists G'.
+    splits.
+    1,2: easy.
+    replace (e_list ++ [e'] ++ e'_list ++ []) with
+        (map (fun (pat_:(e*T)) => match pat_ with (e_,T_) => e_ end )
+           (combine (e_list ++ [e'] ++ e'_list ++[]) (map (fun pat_ : e * T => let (_, T_) := pat_ in T_) e_T_list))).
+    apply typ_func_expr.
+      * intros.
+        rewrite pat2_id in H8.
+        rewrite H3 in H8.
+        rewrite combine_snd in H8.
+        rewrite combine_app in H8...
+        apply in_app_iff in H8.
+        destruct H8.
+        -- apply subG_type with (G1:=G5); auto.
+           apply H2.
+           apply in_map_iff.
+           exists (e_, T_).
+           split; auto.
+           rewrite H3.
+           rewrite combine_app; auto.
+           {
+             eapply in_app_iff.
+             now left.
+           }
+           rewrite 2 app_length.
+           simpl.
+           rewrite H1.
+           reflexivity.
+        -- rewrite combine_app in H8; auto.
+           apply in_app_iff in H8.
+           destruct H8.
+           ++ inv H8;[|contradiction].
+              inv H9.
+              apply H7.
+           ++ apply subG_type with (G1:=G5); auto.
+              apply H2.
+              apply in_map_iff.
+              exists (e_, T_).
+              split; auto.
+              rewrite H3.
+              rewrite combine_app; auto.
+              {
+                eapply in_app_iff.
+                right.
+                right.
+                rewrite app_nil_r in H8.
+                apply H8.
+              }
+           rewrite 2 app_length.
+           simpl.
+           rewrite H1.
+           reflexivity.
+           ++ rewrite app_nil_r.
+              apply H1.
+        -- auto.
+        -- rewrite app_nil_r.
+           simpl.
+           rewrite H1.
+           reflexivity.
+        -- rewrite 4 app_length.
+           simpl.
+           lia.
+      * rewrite combine_snd.
+        ++ apply G'extends.
+           apply H4.
+        ++ rewrite map_length.
+           rewrite H3.
+           rewrite 2 combine_app; auto.
+           ** repeat (rewrite app_length).
+              rewrite 3 combine_length.
+              simpl.
+              rewrite H, H1.
+              lia.
+           ** rewrite 2 app_length.
+              simpl.
+              rewrite H1.
+              reflexivity.
+      * rewrite app_nil_r.
+        rewrite combine_fst; auto.
+        rewrite map_length.
+        rewrite H3.
+        rewrite combine_length.
+        repeat (rewrite app_length).
+        rewrite H, H1.
+        simpl.
+        lia.
+
+  - (* RED_FUN_GROUND *)
+    intros.
+    set (fn_def:=(F_fn T_5 fn5 (map (fun '(T_, x_, _, _) => (T_, x_)) T_x_t_y_list) e5)).
+    pose proof utils.in_split F_list F'_list fn_def .
+    rewrite app_nil_r in *.
+    pose proof Forall_forall (typ_F G5) (F_list ++ [fn_def] ++ F'_list) as (? & _).
+    pose proof H2 F_well_typed fn_def H1 as fn_typed.
+    inv fn_typed.
+    inv e0_type.
+    destruct H as ((?, ?), ?).
+    assert (e_T_list = map (fun '(T_, _, t_, _) => (e_t t_, T_)) T_x_t_y_list).
+    {
+      (* inv H11. *)
+      eapply map_split'.
+      - replace (map fst e_T_list) with (map (fun pat_ : e * T => let (e_, _) := pat_ in e_) e_T_list) by easy.
+        rewrite H4.
+        apply map_ext.
+        easy.
+      - replace (map snd e_T_list) with (map (fun pat_ : e * T => let (_, T_) := pat_ in T_) e_T_list) by easy.
+        rewrite H7 in H11.
+        inv H11.
+        rewrite map_map.
+        apply map_ext.
+        intros.
+        now destruct a as (((?, ?), ?), ?).
+    }
+    exists (fold_right (fun '(T_, _, _, y) G0 => Map.add y (ctxv_T T_) G0) G5 T_x_t_y_list).
+    splits.
+    + eapply fresh_subG; eauto.
+    + rewrite <- fold_map.
+      apply fresh_consistent; eauto.
+      intros.
+      apply in_map_iff in H12.
+      destruct H12 as (Txty, (?, ?)).
+      apply H6.
+      inv H12.
+      rewrite map_map.
+      apply in_map_iff.
+      exists Txty.
+      split; auto.
+      destruct Txty as (((?, ?), ?), ?).
+      now inv H15.
+
+    + rewrite H7 in H11.
+      inv H11.
+      apply subst_lemma; auto.
+      * rewrite <- fold_map_reshuffle; eauto.
+      * rewrite map_xs in H10.
+        apply H10.
+Qed.
+End FunctionalMetatheory.
