theories/utils.v
@@ -1,0 +1,688 @@
+From Coq Require Import List
+  FSets.FMapFacts
+  Lia.
+
+Import ListNotations.
+
+Ltac splits := repeat split.
+Ltac inv H :=inversion H ; subst; clear H.
+Tactic Notation "intros*" := repeat intro.
+
+Ltac forward H :=
+  match type of H with
+  | ?x -> _ =>
+      let name := fresh in assert x as name; [| specialize (H name); clear name]
+  end.
+Tactic Notation "forward" ident(H) :=
+  forward H.
+
+Section ListLemmas.
+  Context {X Y: Type}.
+
+  Lemma map_eq: forall (l: list X) (f g: X -> Y),
+      (forall x, f x = g x) ->
+      map f l = map g l.
+  Proof.
+    induction l; intros; auto.
+    simpl.
+    rewrite (H a).
+    erewrite (IHl); eauto.
+  Qed.
+
+  Lemma map_split {Z W: Type}: forall (l: list (Z*X)) (l2: list (X*Y*Z*W)),
+      map fst l = map (fun '(_, _, z, _) => z) l2 ->
+      map snd l = map (fun '(x, _, _, _) => x) l2 ->
+      l = map (fun '(x, _, z,_) => (z, x)) l2.
+  Proof.
+    induction l; intros.
+    - inv H.
+      symmetry in H2.
+      apply map_eq_nil in H2.
+      now subst.
+    - destruct a.
+      destruct l2.
+      + inv H.
+      + destruct p as (((?, ?), ?), ?).
+        inv H.
+        inv H0.
+        rewrite (IHl l2); auto.
+  Qed.
+
+  Lemma map_xs {Z W: Type}: forall (T_x_t_y_list: list (X*Y*Z*W)),
+      map (fun pat_ : X * Y => let (_, x_) := pat_ in x_) (map (fun '(T_, x_, _, _) => (T_, x_)) T_x_t_y_list) =
+        map (fun '(_, x, _, _) => x) T_x_t_y_list.
+  Proof.
+    induction T_x_t_y_list.
+    - easy.
+    - destruct a as (((?, ?), ?), ?).
+      simpl.
+      now rewrite IHT_x_t_y_list.
+  Qed.
+
+  Lemma map_split' {Z Z' W: Type}: forall (l: list (Z'*X)) (l2: list (X*Y*Z*W)) (f: Z -> Z'),
+      map fst l = map (fun '(_, _, z, _) => f z) l2 ->
+      map snd l = map (fun '(x, _, _, _) => x) l2 ->
+      l = map (fun '(x, _, z,_) => (f z, x)) l2.
+  Proof.
+    induction l; intros.
+    - inv H.
+      symmetry in H2.
+      apply map_eq_nil in H2.
+      now subst.
+    - destruct a.
+      destruct l2.
+      + inv H.
+      + destruct p as (((?, ?), ?), ?).
+        inv H.
+        inv H0.
+        rewrite (IHl l2 f); auto.
+  Qed.
+
+  Lemma combine_fst: forall (l1: list X) (l2: list Y),
+      length l1 = length l2 ->
+      map (fun pat_: (X*Y) => let (e_, _) := pat_ in e_) (combine l1 l2) = l1.
+  Proof.
+    induction l1;intros.
+    - easy.
+    - destruct l2.
+      + inv H.
+      + inv H.
+        simpl.
+        rewrite (IHl1 l2 H1).
+        reflexivity.
+  Qed.
+
+  Lemma combine_nil: forall (l1: list X),
+      @combine X Y l1 [] = [].
+  Proof. destruct l1; easy. Qed.
+
+  Lemma combine_snd: forall (l1: list X) (l2: list Y),
+      length l1 = length l2 ->
+      map (fun pat_: (X*Y) => let (_, e_) := pat_ in e_) (combine l1 l2) = l2.
+  Proof.
+    intros.
+    generalize dependent l1.
+    induction l2; intros.
+    - rewrite combine_nil.
+      auto.
+    - destruct l1.
+      + inv H.
+      + inv H.
+        simpl.
+        rewrite (IHl2 l1 H1).
+        reflexivity.
+  Qed.
+
+  Lemma in_combine: forall (l1: list X) (l2: list Y) x y,
+      In (x,y) (combine l1 l2) -> In x l1 /\ In y l2.
+  Proof.
+    induction l1;intros.
+    - inv H.
+    - destruct l2.
+      + inv H.
+      + destruct H.
+        * inv H.
+          split; left; auto.
+        * destruct (IHl1 l2 x y H).
+          split; right; auto.
+  Qed.
+
+  Lemma combine_app: forall (l1 l2: list X) (l1' l2': list Y),
+      length l1 = length l1' ->
+      length l2 = length l2' ->
+      combine (l1 ++ l2) (l1' ++ l2') = combine l1 l1' ++ combine l2 l2'.
+  Proof.
+    induction l1; intros.
+    - inv H.
+      symmetry in H2.
+      apply length_zero_iff_nil in H2.
+      rewrite H2.
+      easy.
+    - destruct l1'.
+      + inv H.
+      + inv H.
+        simpl.
+        rewrite IHl1; easy.
+  Qed.
+
+  Lemma in_split: forall (l1 l2: list X) x,
+      In x (l1 ++ [x] ++ l2).
+  Proof.
+    induction l1; intros.
+    - left; auto.
+    - right.
+      apply IHl1.
+  Qed.
+
+  Lemma in_combine_split: forall (l: list (X*Y)) l1 l1' l2 l2' x y,
+      length l1 = length l2 ->
+      l = combine (l1 ++ [x] ++ l1') (l2 ++ [y] ++ l2') ->
+      In (x, y) l.
+  Proof.
+    induction l; intros; subst.
+    - destruct l1, l2; easy.
+    - destruct a.
+      destruct l1,l2.
+      + inv H0.
+        left;auto.
+      + inv H.
+      + inv H.
+      + inv H.
+        right.
+        inv H0.
+        eapply IHl.
+        apply H2.
+        reflexivity.
+  Qed.
+
+  Lemma in_fst_iff: forall (l : list (X*Y)) x,
+      (exists y, In (x, y) l) <-> In x (map (fun pat_ : X * Y => let (e_, _) := pat_ in e_) l).
+  Proof.
+    split; intros.
+    - induction l.
+      + destruct H.
+        inv H.
+      + destruct H as (?y & H).
+        inv H.
+        * left; auto.
+        * right.
+          apply IHl.
+          exists y; auto.
+    - induction l.
+      + inv H.
+      + destruct a as (?x & ?y).
+        inv H.
+        * exists y.
+          left;auto.
+        * destruct (IHl H0) as (?y & ?).
+          exists y0.
+          right.
+          apply H.
+  Qed.
+
+  Lemma pat2_id: forall l: list (X*Y),
+      map (fun pat_ : X*Y => let (x_, y_) := pat_ in (x_,y_)) l = l.
+  Proof.
+    induction l;auto.
+    destruct a; cbn.
+    rewrite IHl.
+    reflexivity.
+  Qed.
+
+  Lemma fold_map {A Z W: Type}: forall (f: W -> Z -> A -> A) (l: list (X*Y*Z*W)) a0,
+      fold_right (fun '(_, _, z, w) a => f w z a) a0 l =
+        fold_right (fun (xt : W * Z) a => f (fst xt) (snd xt) a) a0
+          (map (fun pat_ : X*Y*Z*W => let (p, y_) := pat_ in let (p0, t_) := p in let (_, _) := p0 in (y_, t_)) l).
+  Proof.
+    induction l; intros; eauto.
+    destruct a as [[[? ?] ?] ?].
+    simpl.
+    now rewrite IHl.
+  Qed.
+
+  Lemma fold_map1 {A Z W: Type}: forall (f: W -> X -> A -> A) (l: list (X*Y*Z*W)) a0,
+      fold_right (fun '(z, _, _, w) a => f w z a) a0 l =
+        fold_right (fun '(z, w) a => f z w a) a0
+          (map (fun '(z, _, _, w) => (w, z)) l).
+  Proof.
+    induction l; intros; eauto.
+    destruct a as [[[? ?] ?] ?].
+    simpl.
+    now rewrite IHl.
+  Qed.
+
+  Lemma fold_map2 {A Z W: Type}: forall (f: Y -> X -> A -> A) (l: list (X*Y*Z*W)) a0,
+      fold_right (fun '(z, w, _, _) a => f w z a) a0 l =
+        fold_right (fun '(z, w) a => f z w a) a0
+          (map (fun '(z, w, _, _) => (w, z)) l).
+  Proof.
+    induction l; intros; eauto.
+    destruct a as [[[? ?] ?] ?].
+    simpl.
+    now rewrite IHl.
+  Qed.
+
+  Lemma fold_map3 {A Z W: Type}: forall (f: W -> Y -> A -> A) (l: list (X*Y*Z*W)) a0,
+      fold_right (fun '(_, z, _, w) a => f w z a) a0 l =
+        fold_right (fun '(z, w) a => f z w a) a0
+          (map (fun '(_, z, _, w) => (w, z)) l).
+  Proof.
+    induction l; intros; eauto.
+    destruct a as [[[? ?] ?] ?].
+    simpl.
+    now rewrite IHl.
+  Qed.
+
+  Lemma combine_map: forall (l: list (X*Y)),
+      combine (map fst l) (map snd l) = l.
+  Proof.
+    induction l; auto.
+    destruct a; simpl.
+    rewrite IHl.
+    reflexivity.
+  Qed.
+
+  Lemma split_corresponding_list: forall (l: list (X*Y)) left_list mid right_list,
+      map (fun '(x, _) => x) l = left_list ++ [mid] ++ right_list ->
+      exists left_list' mid' right_list',
+        length left_list = length left_list'
+        /\ length right_list = length right_list'
+        /\ l = combine (left_list ++ [mid] ++ right_list) (left_list' ++ [mid'] ++ right_list').
+  Proof with auto.
+    induction l;intros.
+    - apply app_cons_not_nil in H.
+      contradiction.
+    - destruct a.
+      destruct left_list, right_list;
+        inv H.
+      + exists [], y, [].
+        apply map_eq_nil in H2.
+        rewrite H2.
+        splits...
+      + destruct (IHl [] x0 right_list H2)
+          as (left_list' & mid' & right_list' & ? & ? & ?).
+        exists [], y, (left_list' ++ [mid'] ++ right_list').
+        splits...
+        * inv H.
+          symmetry in H4.
+          apply length_zero_iff_nil in H4.
+          rewrite H4.
+          rewrite 2 app_nil_l.
+          rewrite map_length.
+          rewrite combine_length.
+          rewrite 2 app_length.
+          simpl.
+          rewrite H0.
+          lia.
+        * simpl.
+          rewrite H1.
+          rewrite combine_fst.
+          { easy. }
+          rewrite app_nil_l.
+          rewrite 3 app_length.
+          rewrite <- H.
+          rewrite H0.
+          easy.
+      + destruct (IHl left_list mid [] H2)
+          as (left_list' & mid' & right_list' & ? & ? & ?).
+        exists (y::left_list'), mid', right_list'.
+        splits...
+        * inv H0.
+          simpl.
+          rewrite H.
+          easy.
+        * rewrite H1.
+          easy.
+      + destruct (IHl left_list mid (x1::right_list) H2)
+          as (left_list' & mid' & right_list' & ? & ? & ?).
+        exists (y::left_list'), mid', (right_list').
+        splits...
+        * simpl.
+          rewrite H.
+          easy.
+        * rewrite H1.
+          easy.
+  Qed.
+
+  (* I thought this would be useful, but turns out we usually need the length *)
+  Corollary split_corresponding_list_no_length: forall (l: list (X*Y)) left_list mid right_list,
+      map (fun '(x, _) => x) l = left_list ++ [mid] ++ right_list ->
+      exists left_list' mid' right_list', l = combine (left_list ++ [mid] ++ right_list) (left_list' ++ [mid'] ++ right_list').
+  Proof.
+    intros.
+    destruct (split_corresponding_list _ _ _ _ H)
+      as (left_list' & mid' & right_list' & _ & _ & EQ).
+    exists left_list', mid', right_list'.
+    apply EQ.
+  Qed.
+
+End ListLemmas.
+
+Require Import FMapList OrderedTypeEx.
+From ABS Require Import abs_defs.
+From Equations Require Import Equations.
+
+Module MapFacts := FSets.FMapFacts.Facts Map.
+
+
+(* some slightly ad-hoc equalities *)
+Lemma subst_fst_commute: forall x0 x1 e_T_list,
+  map (fun x : e * T => let (e_, _) := let '(e_, T_) := x in (e_var_subst_one e_ x0 x1, T_) in e_) e_T_list =
+  (fix e_list_subst_one (es : list e) (x_ y_ : x) {struct es} : list e :=
+     match es with
+     | [] => fun _ _ : x => []
+     | e :: l => fun x_0 y_0 : x => e_var_subst_one e x_0 y_0 :: e_list_subst_one l x_0 y_0
+     end x_ y_) (map (fun pat_ : e * T => let (e_, _) := pat_ in e_) e_T_list) x0 x1.
+Proof.
+  induction e_T_list; auto.
+  destruct a.
+  simpl.
+  rewrite <- IHe_T_list.
+  reflexivity.
+Qed.
+
+Lemma subst_snd_commutes: forall x0 s e_T_list,
+  map (fun pat_ : e * T => let (_, T_) := pat_ in T_)
+    (map (fun pat_ : e * T => let (e_, T_) := pat_ in (e_var_subst_one e_ x0 s, T_)) e_T_list) =
+    map (fun pat_ : e * T => let (_, T_) := pat_ in T_) e_T_list.
+Proof.
+  intros.
+  induction e_T_list; auto.
+  destruct a;cbn in *.
+  now rewrite IHe_T_list.
+Qed.
+
+(* Characterizing substitution *)
+
+Lemma subst_term: forall t sub,
+  e_var_subst (e_t t) sub = (e_t t).
+Proof.
+  induction sub.
+  - trivial.
+  - destruct a.
+    simpl.
+    rewrite IHsub.
+    now simp e_var_subst_one.
+Qed.
+
+Definition replace_var (x0:x) (sub:list(x*x)) :=
+ fold_right (fun '(x_, y_) x0 => if (eq_x x0 x_) then y_ else x0) x0 sub.
+
+Lemma subst_var: forall x0 sub,
+  e_var_subst (e_var x0) sub = e_var (replace_var x0 sub).
+Proof.
+  induction sub.
+  - trivial.
+  - destruct a; simpl.
+    rewrite IHsub.
+    simp e_var_subst_one.
+    destruct (eq_x (replace_var x0 sub)); subst; eauto.
+Qed.
+
+Lemma e_list_subst_map: forall x0 y0 e_list,
+  e_list_subst_one e_list x0 y0 = map (fun e_ => e_var_subst_one e_ x0 y0) e_list.
+Proof.
+  induction e_list; [easy|];
+  destruct a;
+    simpl;
+    now rewrite IHe_list.
+Qed.
+
+Lemma subst_fn: forall fn0 sub e_list,
+  e_var_subst (e_fn_call fn0 e_list) sub = (e_fn_call fn0 (map (fun e' => e_var_subst e' sub) e_list)).
+Proof.
+  induction sub; intros.
+  - simpl.
+    now rewrite map_id.
+  - destruct a.
+    simpl.
+    rewrite IHsub.
+    simp e_var_subst_one.
+    now rewrite e_list_subst_map, map_map.
+Qed.
+
+Lemma e_list_subst: forall el x0 y0,
+  e_list_subst_one el x0 y0 = map (fun e => e_var_subst_one e x0 y0) el.
+Proof.
+  induction el; intros.
+  - trivial.
+  - simpl.
+    now rewrite IHel.
+Qed.
+
+Lemma e_list_fresh: forall e0 ys el,
+  fresh_vars_el ys el ->
+  In e0 el ->
+  fresh_vars_e ys e0.
+Proof.
+  induction el.
+  - easy.
+  - simpl; intros.
+    destruct H0; subst.
+    + now destruct H.
+    + destruct H.
+      apply IHel; eauto.
+Qed.
+
+(* Properties of fresh_e*)
+Lemma fresh_first_e: forall e0 y ys,
+  fresh_vars_e (y::ys) e0 -> fresh_vars_e [y] e0.
+Proof.
+  induction e0 using e_ott_ind
+    with (P_list_e := fun e_list =>
+                        forall e0 y ys,
+                        In e0 e_list ->
+                        fresh_vars_e (y::ys) e0 -> fresh_vars_e [y] e0);
+     intros; try easy.
+  - simp fresh_vars_e in *.
+    intro.
+    inv H0.
+    + apply H.
+    now left.
+    + inv H1.
+  - simp fresh_vars_e in *.
+    induction e_list.
+    + easy.
+    + inv H.
+      split.
+      * eapply IHe0; eauto.
+        now left.
+      * eapply IHe_list; eauto.
+        intros; eapply IHe0; eauto.
+        now right.
+  - inv H.
+    + eapply IHe0; eauto.
+    + eapply IHe1; eauto.
+Qed.
+
+Lemma fresh_monotone_e: forall e0 y ys,
+  fresh_vars_e (y::ys) e0 -> fresh_vars_e ys e0.
+Proof.
+  induction e0 using e_ott_ind
+    with (P_list_e := fun e_list =>
+                        forall e0 y ys,
+                        In e0 e_list ->
+                        fresh_vars_e (y::ys) e0 -> fresh_vars_e ys e0);
+     intros; try easy.
+  - simp fresh_vars_e in *.
+    intro.
+    apply H.
+    right.
+    assumption.
+  - simp fresh_vars_e in *.
+    induction e_list.
+    + easy.
+    + inv H.
+      split.
+      * eapply IHe0; eauto.
+        now left.
+      * apply IHe_list; eauto.
+        intros; eapply IHe0; eauto.
+        now right.
+  - inv H.
+    + eapply IHe0; eauto.
+    + eapply IHe1; eauto.
+Qed.
+
+Lemma fresh_first_el: forall el y ys,
+    fresh_vars_el (y::ys) el -> fresh_vars_el [y] el.
+Proof.
+  induction el; intros.
+  - now inv H.
+  - inv H.
+    split.
+    + now apply fresh_first_e in H0.
+    + eapply IHel; eauto.
+Qed.
+
+Lemma fresh_monotone_el: forall el y ys,
+  fresh_vars_el (y::ys) el -> fresh_vars_el ys el.
+Proof.
+  induction el; intros.
+  - now inv H.
+  - inv H.
+    split.
+    + now apply fresh_monotone_e in H0.
+    + eapply IHel; eauto.
+Qed.
+
+Lemma fresh_var_subst: forall e0 y sub,
+  fresh_vars_e (map snd sub) e0 ->
+  fresh_vars_e [y] e0 ->
+  ~ In y (map snd sub) ->
+  fresh_vars_e [y] (e_var_subst e0 sub).
+Proof.
+  intros.
+  generalize dependent y.
+  generalize dependent e0.
+  induction e0 using e_ott_ind
+    with
+    (P_list_e := fun e_list => forall y,
+                     fresh_vars_el (map snd sub) e_list ->
+                     fresh_vars_el [y] e_list ->
+                     ~ In y (map snd sub) ->
+                     fresh_vars_el [y] (map (fun e' => e_var_subst e' sub) e_list))
+  ; intros; auto.
+  - rewrite subst_term.
+    now simp e_var_subst_one.
+  - induction sub; auto.
+    destruct a as (?x_, ?y); simpl.
+    rewrite subst_var.
+    simp e_var_subst_one.
+    destruct (eq_x (replace_var x5 sub) x_).
+    + simp fresh_vars_e.
+      intro.
+      apply H1.
+      left.
+      now inv H2.
+    + rewrite <- subst_var.
+      apply Decidable.not_or in H1.
+      destruct H1.
+      apply fresh_monotone_e in H.
+      eapply IHsub; auto.
+  - rewrite subst_fn.
+    simp fresh_vars_e in *.
+  - destruct H,H0.
+    split.
+    + apply IHe0; auto.
+    + apply IHe1; eauto.
+Qed.
+
+Fact disjoint_empty{A:Type}: @disjoint A [] [].
+Proof. easy. Qed.
+
+Lemma disjoint_monotone {A:Type}: forall (l1 l2: list A) a1 a2,
+  disjoint (a1::l1) (a2::l2) -> disjoint l1 l2.
+Proof.
+  intros.
+  intros ? ? ?.
+    specialize (H a).
+    apply H; now right.
+Qed.
+
+Section MapLemmas.
+
+  Lemma map_neq_none_is_some{elt:Type}: forall m x,
+      Map.find x m <> None ->
+      exists y, Map.find (elt:=elt) x m = Some y.
+  Proof.
+    intros.
+    destruct (MapFacts.In_dec m x).
+    - inv i.
+      exists x0.
+      apply Map.find_1.
+      apply H0.
+    - apply MapFacts.not_find_in_iff in n.
+      rewrite n in H.
+      contradiction.
+  Qed.
+
+  Lemma fold_map_reshuffle: forall (l: list (T*x*t*x)) G0,
+      (fold_right (fun (ax : x * T) (G' : G) => Map.add (fst ax) (ctxv_T (snd ax)) G') G0
+         (map (fun pat_ : T * x => let (T_, x_) := pat_ in (x_, T_)) (map (fun '(T_0, x_, _, _) => (T_0, x_)) l)))
+      = (fold_right (fun '(T1, x_, _, _) (G' : G) => Map.add x_ (ctxv_T T1) G') G0 l).
+  Proof.
+    induction l;intros;auto.
+    destruct a as (((?T_ & ?x_) & ?t_) & ?y).
+    simpl.
+    rewrite IHl.
+    reflexivity.
+  Qed.
+
+  Lemma map_add_comm{E:Type}: forall m key key' elt elt',
+      key <> key' -> Map.Equal (Map.add (elt:=E) key elt (Map.add key' elt' m)) (Map.add key' elt' (Map.add key elt m)).
+  Proof.
+    intros.
+    intro.
+    destruct (Map.find y m) eqn:?.
+    - destruct (eq_x y key), (eq_x y key'); subst;
+        erewrite 2 Map.find_1; eauto;
+        (* this should just be "eauto with map", but I can't seem to import the hint database *)
+        try (apply Map.add_2; eauto; now apply Map.add_1);
+        try (now apply Map.add_1; eauto);
+        try (repeat (apply Map.add_2; eauto); now apply Map.find_2; eauto).
+    - destruct (eq_x y key), (eq_x y key'); subst.
+      + contradiction.
+      + erewrite 2 Map.find_1; eauto.
+        * apply Map.add_2; eauto.
+          now apply Map.add_1.
+        * now apply Map.add_1.
+      + erewrite 2 Map.find_1; eauto.
+        * now apply Map.add_1.
+        * apply Map.add_2; eauto.
+          now apply Map.add_1.
+
+      (* there has to be a cleaner way to do this case?? *)
+      + replace (Map.find (elt:=E) y (Map.add key elt (Map.add key' elt' m))) with (@None E).
+        replace (Map.find (elt:=E) y (Map.add key' elt' (Map.add key elt m))) with (@None E).
+        reflexivity.
+        * symmetry.
+          apply MapFacts.not_find_in_iff in Heqo.
+          apply MapFacts.not_find_in_iff.
+          intro.
+          apply Heqo.
+          inv H0.
+          exists x.
+          apply Map.add_3  with (x:= key) (e':=elt); auto.
+          apply Map.add_3 with (x:=key') (e':=elt'); auto.
+        * symmetry.
+          apply MapFacts.not_find_in_iff in Heqo.
+          apply MapFacts.not_find_in_iff.
+          intro.
+          inv H0.
+          apply Heqo.
+          exists x.
+          apply Map.add_3 with (x:=key') (e':=elt'); auto.
+          apply Map.add_3  with (x:= key) (e':=elt); auto.
+  Qed.
+
+  Lemma fold_not_in: forall G0 y (T_x_t_y_list: list (T*x*t*x)),
+      ~ Map.In y G0 ->
+      ~ In y (map (fun '(_, _, _, y') => y') T_x_t_y_list) ->
+      ~ Map.In y (fold_right (fun '(T_, _, _, y) (G0 : G) => Map.add y (ctxv_T T_) G0) G0 T_x_t_y_list).
+  Proof.
+    induction T_x_t_y_list as [ | (((?T_, ?x_), ?t_), ?y) T_x_t_y_list IH ]; [easy|].
+    simpl; intros ? ? ?.
+    destruct (eq_x y y0); subst.
+    - apply H0.
+      now left.
+    - apply MapFacts.add_in_iff in H1.
+      inv H1.
+      + apply H0.
+        now left.
+      + apply IH; eauto.
+  Qed.
+
+  Lemma fold_add_comm: forall G0 y T_ (upd: list (T*x)),
+      ~ In y (map (fun '(_, y) => y) upd) ->
+      Map.Equal (Map.add y (ctxv_T T_) (fold_right (fun '(T_, y) G0 => Map.add y (ctxv_T T_) G0) G0 upd))
+        (fold_right (fun '(T_, y) G0 => Map.add y (ctxv_T T_) G0) (Map.add y (ctxv_T T_) G0) upd).
+  Proof.
+    induction upd; intros.
+    - easy.
+    - destruct a; simpl in *.
+      apply Decidable.not_or in H.
+      destruct H.
+      now rewrite map_add_comm, IHupd; auto.
+  Qed.
+End MapLemmas.
